InferenceInLean/Exercises.lean
@@ -7,13 +7,11 @@ open Syntax
 open Semantics
 open Models
 open Unification
-open Inference
+open Inferences
 
 namespace Examples
 
-/-
-### Example Peano Arithmetic
--/
+/- ### Example Peano Arithmetic -/
 
 inductive PeanoFuns where
   | zero
@@ -23,6 +21,7 @@ inductive PeanoFuns where
 
 inductive PeanoPreds where
   | less_than
+  | eq
 
 @[simp]
 def ex_sig_peano : Signature := ⟨PeanoFuns, PeanoPreds⟩
@@ -35,12 +34,11 @@ def ex_formula_peano : @Formula ex_sig_peano String :=
   .all "x" <| .all "y" <| .iff
     (.or
       (.atom (.pred .less_than [.var "x", .var "y"]))
-      (.atom (.eq (.var "x") (.var "y"))))
-    (.ex "z" (.atom (.eq (.func .add [.var "x", .var "z"]) (.var "y"))))
+      (.atom (.pred .eq [(.var "x"), (.var "y")])))
+    (.ex "z" (.atom (.pred .eq [(.func .add [.var "x", .var "z"]), (.var "y")])))
 
 @[simp]
-def ex_interpret_peano : Interpretation ex_sig_peano where
-  univ := ℕ
+def ex_interpret_peano : Interpretation ex_sig_peano ℕ where
   functions := λ
     | .zero => λ _ => 0
     | .succ => λ xs => xs[0]! + 1
@@ -48,6 +46,7 @@ def ex_interpret_peano : Interpretation ex_sig_peano where
     | .mul => λ xs => xs[0]! * xs[1]!
   predicates := λ f => match f with
     | .less_than => λ xs => xs[0]! < xs[1]!
+    | .eq => λ xs => xs[0]! = xs[1]!
 
 def ex_assig_peano : Assignment String Nat
   | "x" => 0
@@ -61,19 +60,19 @@ def example_substitution : Substitution ex_sig_peano String := λ x => match x w
 def ex_formula_peano_lt : @Formula ex_sig_peano String :=
   .all "z" (.atom $ .pred .less_than [.var "x", .func .succ [.func .succ [.var "z"]]])
 
-lemma ex_proof_lt : @Formula.eval ex_sig_peano String instDecidableEqString
+lemma ex_proof_lt : @Formula.eval ex_sig_peano String ℕ instDecidableEqString
     ex_interpret_peano ex_assig_peano ex_formula_peano_lt := by
   simp [ex_formula_peano_lt, ex_sig_peano, Interpretation, Assignment, ex_assig_peano]
 
 
-#eval @Term.eval ex_sig_peano String ex_interpret_peano ex_assig_peano (Term.var "y")
+#eval @Term.eval ex_sig_peano String ℕ ex_interpret_peano ex_assig_peano (Term.var "y")
 
 def ex_term_peano : Term ex_sig_peano String :=
     Term.func .add [Term.var "x", Term.var "y"]
 
-#eval @Term.eval ex_sig_peano String ex_interpret_peano ex_assig_peano ex_term_peano
+#eval @Term.eval ex_sig_peano String ℕ ex_interpret_peano ex_assig_peano ex_term_peano
 
-lemma ex_peano_proof: @Formula.eval ex_sig_peano String instDecidableEqString
+lemma ex_peano_proof: @Formula.eval ex_sig_peano String ℕ instDecidableEqString
     ex_interpret_peano ex_assig_peano ex_formula_peano := by
   simp
   intro a b
@@ -92,33 +91,29 @@ lemma ex_peano_proof: @Formula.eval ex_sig_peano String instDecidableEqString
     exact Or.symm (Nat.eq_zero_or_pos z)
 
 def exa : Formula ex_sig_peano String := .and .falsum .verum
-example : ¬@Formula.eval ex_sig_peano _ _ ex_interpret_peano ex_assig_peano exa :=
+example : ¬@Formula.eval ex_sig_peano _ _ _ ex_interpret_peano ex_assig_peano exa :=
   of_eq_true (Eq.trans (congrArg Not (and_true False)) not_false_eq_true)
 
-
-example : @EntailsInterpret ex_sig_peano String _ ex_interpret_peano
+example : @EntailsInterpret ex_sig_peano String _ _ ex_interpret_peano
   ex_assig_peano ex_formula_peano := ex_peano_proof
 
 
+variable {sig : Signature} {X : Variables} {univ : Universes}
 /-
 Proposition 3.3.3 Let F and G be formulas, let N be a set of formulas. Then
 (i) F is valid if and only if ¬F is unsatisfiable.
 (ii) F |= G if and only if F ∧ ¬G is unsatisfiable.
--/
-theorem valid_iff_not_unsat {sig : Signature} {X : Variables} [inst : DecidableEq X]
-    (F : Formula sig X) : Valid F ↔ @Unsatisfiable sig X inst (Formula.neg F) := by simp
-
-theorem entails_iff_and_not_unsat {sig : Signature} {X : Variables} [inst : DecidableEq X]
-    (F G : Formula sig X) :
-    Entails F G ↔ @Unsatisfiable sig X inst (Formula.and F (Formula.neg G)) := by simp
-
-/-
--- TODO: finish this proof
 (iii) N |= G if and only if N ∪ {¬G} is unsatisfiable.
 -/
-theorem setEntails_iff_union_not_unsat {sig : Signature} {X : Variables} [inst : DecidableEq X]
+theorem valid_iff_not_unsat' [inst : DecidableEq X] (F : Formula sig X) :
+    @Valid _ _ univ _ F ↔ @Unsatisfiable _ _ univ _ (Formula.neg F) := by simp
+
+theorem entails_iff_and_not_unsat' [inst : DecidableEq X] (F G : Formula sig X) :
+    @Entails _ _ univ _ F G ↔ @Unsatisfiable _ _ univ _ (Formula.and F (Formula.neg G)) := by simp
+
+theorem setEntails_iff_union_not_unsat' [inst : DecidableEq X]
     (N : Set $ Formula sig X) (G : Formula sig X) :
-    SetEntails N G ↔ @SetUnsatisfiable sig X inst (N ∪ {Formula.neg G}) := by
+    @SetEntails _ _ univ _ N G ↔ @SetUnsatisfiable _ _ univ _ (N ∪ {Formula.neg G}) := by
   apply Iff.intro
   · intro hentails I β
     simp_all only [SetEntails, Assignment, EntailsInterpret, Set.union_singleton,
@@ -132,6 +127,31 @@ theorem setEntails_iff_union_not_unsat {sig : Signature} {X : Variables} [inst :
     aesop
 
 
+/- ## Exercise 4 -/
+
+namespace Exercise4
+
+/- ### Exercise 4-1 -/
+
+inductive fs where | b | c | d | f deriving BEq
+inductive ps where | P
+def F : Formula ⟨fs, ps⟩ String := .and (.and (.and (.atom (.pred .P [.func .b []]))
+  (.atom (.pred .P [.func .c []])))
+  (.neg (.atom (.pred .P [.func .d []]))))
+  (.neg (.ex "x" (.atom (.pred .P [.func .f [.func .f [.var "x"]]]))))
+
+theorem ex_4_1 : ∃ I : Interpretation ⟨fs, ps⟩ (Fin 2), ∃ β : Assignment String (Fin 2),
+    Formula.eval I β F := by
+  let I : Interpretation ⟨fs, ps⟩ (Fin 2) := ⟨
+    fun g a => if g == .f || g == .d then 1 else 0,
+    fun _ u => if u[0]! == 0 then True else False⟩
+  use I
+  use (fun _ => 0)
+  simp [I, F]
+  have : fs.f == fs.f := rfl
+  aesop
+
+
 /-
 Exercise 4.7 (*)
 Let Π be a set of propositional variables. Let N and N' be sets
@@ -140,86 +160,63 @@ literals. Prove: If every clause in N contains at least one literal L with L ∈
 clause in N' contains a literal L with L ∈ S, then N ∪ N' is satisfiable if and only if N'
 is satisfiable.
 -/
-theorem ex_4_7 {sig : Signature} {X : Variables} [DecidableEq X]
-    (N N' : Set $ Clause sig X) (S : Set $ Literal sig X)
+def Interpretation.add (I : Interpretation ⟨Empty, String⟩ String)
+    (β : Assignment Empty String) (L : Literal ⟨Empty, String⟩ Empty) :
+    Interpretation ⟨Empty, String⟩ String :=
+  -- add something to I such that Formula.eval L is true
+  Interpretation.mk I.functions (match L with
+    | Literal.pos a => match a with
+      | Atom.pred p args =>
+        have argsinter := args.map (Term.eval I β)
+        (fun p' args' => if p' == p && args' == argsinter
+          then True
+          else I.predicates p' args')
+    | Literal.neg a => match a with
+      | Atom.pred p args =>
+        have argsinter := args.map (Term.eval I β)
+        (fun p' args' => if p' == p && args' == argsinter
+          then False
+          else I.predicates p' args')
+  )
+
+lemma tmp (I : Interpretation ⟨Empty, String⟩ String) (β : Assignment Empty String)
+    (C : Clause ⟨Empty, String⟩ Empty)
+    (hCsat : EntailsInterpret I β C) (L : Literal ⟨Empty, String⟩ Empty) (h : L.comp ∉ C) :
+    EntailsInterpret (Interpretation.add I β L) β C := by
+  sorry
+
+theorem ex_4_7
+    (N N' : Set <| Clause ⟨Empty, String⟩ Empty) (S : Set <| Literal ⟨Empty, String⟩ Empty)
     (hSnoCompl : ∀ L ∈ S, L.comp ∉ S)
-    (hNsatByS : ∀ C ∈ N, ∃ L ∈ C, L ∈ S) (hN'noComplS : ∀ C ∈ N', ∀ L ∈ C, L ∉ S) :
-    (ClauseSetSatisfiable (N ∪ N') ↔ ClauseSetSatisfiable N') := by
+    (hNsatByS : ∀ C ∈ N, ∃ L ∈ C, L ∈ S) (hN'noComplS : ∀ C ∈ N', ¬∃ L ∈ C, L.comp ∈ S) :
+    (@ClauseSetSatisfiable _ _ univ _ (N ∪ N') ↔ @ClauseSetSatisfiable _ _ univ _ N') := by
+  simp only [not_exists, not_and] at hN'noComplS
   apply Iff.intro
   · simp [ClauseSetSatisfiable]
-    intro I β
-    intro h
+    intro I β h
     apply Exists.intro
     · apply Exists.intro
       · intro C a
         apply h
         simp_all only [or_true]
   · simp [ClauseSetSatisfiable]
-    intro I_N' β_N'
-    intro hN'sat
+    intro I_N' β_N' hN'sat
     use I_N'
-    use β_N'
+    use β_N' -- delay instanciation of assignment
     intro C hC
     cases hC
-    /- This is the actual hard case of this exercise. On paper it might look like this:
-        - Show that I_N' and β_N' do not contradict (SAT N) (this is due to hN'noComplS)
-        - Expand β_N' by the assignments implied by S to β_N'andS
-        - then β_N'andS satisfies N using hNsatByS
-    -/
-    next h => sorry
-    next h => exact hN'sat C h
+    next hCinN =>
+      /- This is the actual hard case of this exercise. On paper it might look like this:
+          - Show that I_N' and β_N' do not contradict (SAT N) (this is due to hN'noComplS)
+          - Expand β_N' by the assignments implied by S to β_N'andS
+          - then β_N'andS satisfies N using hNsatByS
+      -/
+      obtain ⟨L, ⟨hLinC, hLinS⟩⟩ := hNsatByS C hCinN
+      have hLcompninS : L.comp ∉ S := by exact hSnoCompl L hLinS
+      --let ?β := β_N'
+      --let β_N'andS := β.modify L
+      sorry
 
-/--
-Example for the proof type with resolution.
-TODO: Finish this
--/
-inductive ExFuns
-| b
-| c
-| f
-| h
+    next hCinN' => exact hN'sat C hCinN'
 
-inductive ExPreds
-| P
-| Q
-
-def ex_sig_ground : Signature := ⟨ExFuns, ExPreds⟩
-
-def ex_clause : Clause ex_sig_ground Empty :=
-  [.pos (Atom.pred .P [.func ExFuns.b []]),
-   .pos (Atom.pred .P [.func ExFuns.b []])]
-
-def ex_clause' : Clause ex_sig_ground Empty :=
-  [.neg (Atom.pred .P [.func ExFuns.b []])]
-
-def ex_conc : Clause ex_sig_ground Empty :=
-  [.pos (Atom.pred .P [.func ExFuns.b []])]
-
--- forget about that, the rules are schematic but we don't have that notion here
-def example_proof {A : @Atom ex_sig_ground Empty} {C D : @Clause ex_sig_ground Empty} :
-    @Proof ex_sig_ground Empty (@Resolution.GroundResolution ex_sig_ground A D C) := {
-      assumptions := {ex_clause}
-      clauses := [ex_clause, ex_conc]
-      conclusion := ex_conc
-      clauses_not_empty := by simp
-      last_clause_conclusion := by simp
-      is_valid := by
-        simp only [List.length_cons, List.length_singleton, Nat.reduceAdd, Set.mem_insert_iff,
-          Set.mem_singleton_iff]
-        simp_all
-        intro i hle
-        have : i = 0 ∨ i = 1 := by sorry
-        cases this
-        next h => simp [h]
-        next h =>
-          subst h
-          apply Or.inr
-          have fact : Inference ex_sig_ground Empty := {
-            premises := {ex_clause}
-            conclusion := ex_conc
-          }
-          use fact
-          apply And.intro
-          · sorry
-          · sorry
-    }
+end Exercise4
